SimplifyTargeted proofs

coq/SimpleForm/Simplifications/SimplifyTargeted.v
@@ -128,30 +128,20 @@ Section SimplifyTargeted.
   : sact :=
     simplify_sact_targeted_aux ua exemptions [].
 
-  Definition simplify_sf_targeted
-    (sf: simple_form) (exemptions: list (list position))
-  := {|
-    final_values := final_values sf;
-    vars :=
-      fst (
-        PTree.fold
-        (fun
-          (acc: ((PTree.tree (type * SimpleForm.sact)) * list (list position)))
-          elt (val: (type * SimpleForm.sact))
-        =>
-          let '(tree, acc_exs) := acc in
-          let exs: list position := List.hd [] acc_exs in
-          let res := simplify_sact_targeted (snd val) exs in
-          (PTree.set elt (fst val, res) tree, tl acc_exs))
-        (vars sf)
-        (PTree.empty (type * SimpleForm.sact), exemptions))
-    |}.
 
   Lemma simplify_targeted_no_exemptions_pos_irrelevant:
     forall a p1 p2,
     simplify_sact_targeted_aux a [] p1 = simplify_sact_targeted_aux a [] p2.
   Proof.
-  Admitted.
+    induction a; simpl; intros; eauto.
+    - rewrite IHa1 with (p2:=branch1::p2).
+      rewrite IHa2 with (p2:=branch2::p2).
+      rewrite IHa3 with (p2:=branch3::p2). auto.
+    - rewrite IHa with (p2:=branch1::p2). auto.
+    - rewrite IHa1 with (p2:=branch1::p2).
+      rewrite IHa2 with (p2:=branch2::p2). auto.
+    - rewrite IHa with (p2:=branch1::p2). auto.
+  Qed.
 
   Lemma sact_simplify_targeted_no_exemptions_eq_simplify :
     forall a,
@@ -170,28 +160,30 @@ Section SimplifyTargeted.
       erewrite simplify_targeted_no_exemptions_pos_irrelevant in IHa1.
       erewrite simplify_targeted_no_exemptions_pos_irrelevant in IHa2.
       rewrite IHa1, IHa2. eauto.
-    (* - unfold simplify_sact_targeted in *. simpl. *)
-    (*   erewrite simplify_targeted_no_exemptions_pos_irrelevant in IHa. *)
-    (*   rewrite IHa. eauto. *)
-  Admitted.
+    - unfold simplify_sact_targeted in *. simpl.
+      erewrite simplify_targeted_no_exemptions_pos_irrelevant in IHa.
+      rewrite IHa. eauto.
+  Qed.
 
-  Lemma simplify_targeted_no_exemptions_eq_simplify :
-    forall sf,
-    simplify_sf_targeted sf [] = simplify_sf r sigma sf.
-  Proof.
-    intros.
-    destruct sf.
-    unfold simplify_sf, simplify_sf_targeted.
-    simpl. f_equal.
-    unfold simplify_vars.
-    f_equal.
-    (* apply functional_extensionality; intro. *)
-    (* apply functional_extensionality; intro. *)
-    (* destruct x0. simpl. *)
-    (* f_equal. *)
-    (* destruct (Pos.to_nat x); *)
-    (*   apply sact_simplify_targeted_no_exemptions_eq_simplify. *)
-  Admitted.
+  (* Lemma simplify_targeted_no_exemptions_eq_simplify : *)
+  (*   forall sf, *)
+  (*   simplify_sf_targeted sf [] = simplify_sf r sigma sf. *)
+  (* Proof. *)
+  (*   intros. *)
+  (*   destruct sf. *)
+  (*   unfold simplify_sf, simplify_sf_targeted. *)
+  (*   simpl. f_equal. *)
+  (*   unfold simplify_vars. *)
+  (*   rewrite PTree.fold_spec. simpl. *)
+
+  (*   f_equal. *)
+  (*   (* apply functional_extensionality; intro. *) *)
+  (*   (* apply functional_extensionality; intro. *) *)
+  (*   (* destruct x0. simpl. *) *)
+  (*   (* f_equal. *) *)
+  (*   (* destruct (Pos.to_nat x); *) *)
+  (*   (*   apply sact_simplify_targeted_no_exemptions_eq_simplify. *) *)
+  (* Admitted. *)
 
   Lemma simplify_unop_targeted_cases:
     forall e p ufn a a',
@@ -201,138 +193,546 @@ Section SimplifyTargeted.
     -> (
       exists b x,
       eval_sact_no_vars
-        r sigma (simplify_sact_targeted_aux a e (p ++ [branch1]))
+        r sigma (simplify_sact_targeted_aux a e (branch1 :: p))
       = Some b
       /\ sigma1 ufn b = Some x
       /\ a' = SConst x)
-    \/ a' = SUnop ufn (simplify_sact_targeted_aux a e (p ++ [branch1])).
+    \/ a' = SUnop ufn (simplify_sact_targeted_aux a e (branch1 :: p)).
   Proof.
-  Admitted.
+    simpl. intros.
+    destr_in H; subst. right; auto.
+    destr. 2: right; auto.
+    destr. left; do 2 eexists; repeat split; eauto.
+    right; auto.
+  Qed.
 
   Lemma simplify_bnop_targeted_cases:
     forall ufn a1 a2 a' e p,
     simplify_sact_targeted_aux (SBinop ufn a1 a2) e p = a'
-    -> a' = SBinop ufn (simplify_sact_targeted_aux a1 e (p ++ [branch1])) (simplify_sact_targeted_aux a2 e (p ++ [branch2]))
+    -> a' = SBinop ufn (simplify_sact_targeted_aux a1 e (branch1 :: p)) (simplify_sact_targeted_aux a2 e (branch2 :: p))
     \/ (ufn = PrimUntyped.UBits2 PrimUntyped.UAnd
-      /\ ((eval_sact_no_vars r sigma (simplify_sact_targeted_aux a1 e (p ++ [branch1])) = Some (Bits [true])
-        /\ a' = simplify_sact_targeted_aux a2 e (p ++ [branch2]))
-        \/ (eval_sact_no_vars r sigma (simplify_sact_targeted_aux a1 e (p ++ [branch1])) = Some (Bits [false])
+      /\ ((eval_sact_no_vars r sigma (simplify_sact_targeted_aux a1 e (branch1 :: p)) = Some (Bits [true])
+        /\ a' = simplify_sact_targeted_aux a2 e (branch2 :: p))
+        \/ (eval_sact_no_vars r sigma (simplify_sact_targeted_aux a1 e (branch1 :: p)) = Some (Bits [false])
           /\ a' = const_false)
-        \/ (eval_sact_no_vars r sigma (simplify_sact_targeted_aux a2 e (p ++ [branch2])) = Some (Bits [true])
-            /\ a' = simplify_sact_targeted_aux a1 e (p ++ [branch1]))
-        \/ (eval_sact_no_vars r sigma (simplify_sact_targeted_aux a2 e (p ++ [branch2])) = Some (Bits [false])
+        \/ (eval_sact_no_vars r sigma (simplify_sact_targeted_aux a2 e (branch2 :: p)) = Some (Bits [true])
+            /\ a' = simplify_sact_targeted_aux a1 e (branch1 :: p))
+        \/ (eval_sact_no_vars r sigma (simplify_sact_targeted_aux a2 e (branch2 :: p)) = Some (Bits [false])
             /\ a' = const_false)))
     \/ (ufn = PrimUntyped.UBits2 PrimUntyped.UOr
-        /\ ((eval_sact_no_vars r sigma (simplify_sact_targeted_aux a1 e (p ++ [branch1])) = Some (Bits [true])
+        /\ ((eval_sact_no_vars r sigma (simplify_sact_targeted_aux a1 e (branch1 :: p)) = Some (Bits [true])
              /\ a' = const_true)
-            \/ (eval_sact_no_vars r sigma (simplify_sact_targeted_aux a1 e (p ++ [branch1])) = Some (Bits [false])
-                /\ a' = simplify_sact_targeted_aux a2 e (p ++ [branch2]))
-            \/ (eval_sact_no_vars r sigma (simplify_sact_targeted_aux a2 e (p ++ [branch2])) = Some (Bits [true])
+            \/ (eval_sact_no_vars r sigma (simplify_sact_targeted_aux a1 e (branch1 :: p)) = Some (Bits [false])
+                /\ a' = simplify_sact_targeted_aux a2 e (branch2 :: p))
+            \/ (eval_sact_no_vars r sigma (simplify_sact_targeted_aux a2 e (branch2 :: p)) = Some (Bits [true])
                 /\ a' = const_true)
-            \/ (eval_sact_no_vars r sigma (simplify_sact_targeted_aux a2 e (p ++ [branch2])) = Some (Bits [false])
-                /\ a' = simplify_sact_targeted_aux a1 e (p ++ [branch1]))))
+            \/ (eval_sact_no_vars r sigma (simplify_sact_targeted_aux a2 e (branch2 :: p)) = Some (Bits [false])
+                /\ a' = simplify_sact_targeted_aux a1 e (branch1 :: p))))
   \/ (
     exists v1 v2 v,
-    eval_sact_no_vars r sigma (simplify_sact_targeted_aux a1 e (p ++ [branch1])) = Some v1
-    /\ eval_sact_no_vars r sigma (simplify_sact_targeted_aux a2 e (p ++ [branch2])) = Some v2
+    eval_sact_no_vars r sigma (simplify_sact_targeted_aux a1 e (branch1 :: p)) = Some v1
+    /\ eval_sact_no_vars r sigma (simplify_sact_targeted_aux a2 e (branch2 :: p)) = Some v2
     /\ sigma2 ufn v1 v2 = Some v
     /\ a' = SConst v).
   Proof.
-  Admitted.
+    simpl. intros.
+    destr_in H; subst. auto.
+    destr.
+    destr; try destr; try destr; auto. (repeat right; do 3 eexists; repeat split; eauto; auto).
+    destr.
+    repeat destr; intuition eauto.
+    repeat destr; intuition eauto.
+    {
+    repeat destr; intuition eauto.
+    (repeat right; do 3 eexists; repeat split; eauto; auto).
+    }
+    repeat destr; intuition eauto;     (repeat right; do 3 eexists; repeat split; eauto; auto).
+    repeat destr; intuition eauto;     (repeat right; do 3 eexists; repeat split; eauto; auto).
+    repeat destr; intuition eauto;     (repeat right; do 3 eexists; repeat split; eauto; auto).
+    repeat destr; intuition eauto;     (repeat right; do 3 eexists; repeat split; eauto; auto).
+    repeat destr; intuition eauto;     (repeat right; do 3 eexists; repeat split; eauto; auto).
+    repeat destr; intuition eauto;     (repeat right; do 3 eexists; repeat split; eauto; auto).
+    repeat destr; intuition eauto;     (repeat right; do 3 eexists; repeat split; eauto; auto).
+    repeat destr; intuition eauto;     (repeat right; do 3 eexists; repeat split; eauto; auto).
+    repeat destr; intuition eauto;     (repeat right; do 3 eexists; repeat split; eauto; auto).
+    repeat destr; intuition eauto;     (repeat right; do 3 eexists; repeat split; eauto; auto).
+    repeat destr; intuition eauto;     (repeat right; do 3 eexists; repeat split; eauto; auto).
+    repeat destr; intuition eauto;     (repeat right; do 3 eexists; repeat split; eauto; auto).
+    repeat destr; intuition eauto;     (repeat right; do 3 eexists; repeat split; eauto; auto).
+  Qed.
 
-  Lemma simplify_sact_targeted_correct:
-    forall vvs (WTV: wt_vvs R (Sigma:=Sigma) vvs) n a res t e p,
-    wt_sact (Sigma:=Sigma) R vvs a t
-    -> eval_sact vvs a n = Some res
-    -> eval_sact vvs (simplify_sact_targeted_aux a e p) n = Some res.
-  Proof.
-  Admitted.
+  Definition eval_sact_no_vars_bool (ex: bool) a :=
+    if ex then None else
+    match eval_sact_no_vars r sigma a with
+    | Some (Bits [true]) => Some true
+    | Some (Bits [false]) => Some false
+    | _ => None
+    end.
 
-  Lemma simpl_sact_targeted_aux_some_p1_p2:
-    forall e a p1 p2 v1 v2,
-    eval_sact_no_vars r sigma (simplify_sact_targeted_aux a e p1) = Some v1
-    -> eval_sact_no_vars r sigma (simplify_sact_targeted_aux a e p2) = Some v2
-    -> v1 = v2.
+  Inductive ssta : sact -> list position -> position -> sact -> Prop :=
+  | ssta_if_true:
+    forall c tb fb e pos tc ttb,
+      ssta c e (branch1 :: pos) tc ->
+      eval_sact_no_vars r sigma tc = Some (Bits [true]) ->
+      ssta tb e (branch2 :: pos) ttb ->
+      ssta (SIf c tb fb) e pos ttb
+  | ssta_if_false:
+    forall c tb fb e pos tc tfb,
+      ssta c e (branch1 :: pos) tc ->
+      eval_sact_no_vars r sigma tc = Some (Bits [false]) ->
+      ssta fb e (branch3 :: pos) tfb ->
+      ssta (SIf c tb fb) e pos tfb
+  | ssta_if_exempted:
+    forall c tb fb e pos tc ttb tfb,
+      ssta c e (branch1 :: pos) tc ->
+      ssta tb e (branch2 :: pos) ttb ->
+      ssta fb e (branch3 :: pos) tfb ->
+      ssta (SIf c tb fb) e pos (SIf tc ttb tfb)
+  | ssta_unop:
+    forall ufn a e pos ta v v1,
+      ssta a e (branch1 :: pos) ta ->
+      eval_sact_no_vars r sigma ta = Some v ->
+      sigma1 ufn v = Some v1 ->
+      ssta (SUnop ufn a) e pos (SConst v1)
+  | ssta_unop_exempted:
+    forall ufn a e pos ta,
+      ssta a e (branch1 :: pos) ta ->
+      ssta (SUnop ufn a) e pos (SUnop ufn ta)
+  | ssta_binop_and_true_:
+    forall a e pos ta b tb,
+      ssta a e (branch1::pos) ta ->
+      eval_sact_no_vars r sigma ta = Some (Bits [true]) ->
+      ssta b e (branch2::pos) tb ->
+      ssta (SBinop (PrimUntyped.UBits2 PrimUntyped.UAnd) a b) e pos tb
+  | ssta_binop_and_false_:
+    forall a e pos ta b,
+      ssta a e (branch1::pos) ta ->
+      eval_sact_no_vars r sigma ta = Some (Bits [false]) ->
+      ssta (SBinop (PrimUntyped.UBits2 PrimUntyped.UAnd) a b) e pos const_false
+  | ssta_binop_and__true:
+    forall a e pos ta b tb,
+      ssta a e (branch1::pos) ta ->
+      ssta b e (branch2::pos) tb ->
+      eval_sact_no_vars r sigma tb = Some (Bits [true]) ->
+      ssta (SBinop (PrimUntyped.UBits2 PrimUntyped.UAnd) a b) e pos ta
+  | ssta_binop_and__false:
+    forall a e pos b tb,
+      ssta b e (branch2::pos) tb ->
+      eval_sact_no_vars r sigma tb = Some (Bits [false]) ->
+      ssta (SBinop (PrimUntyped.UBits2 PrimUntyped.UAnd) a b) e pos const_false
+  | ssta_binop_or_false_:
+    forall a e pos ta b tb,
+      ssta a e (branch1::pos) ta ->
+      eval_sact_no_vars r sigma ta = Some (Bits [false]) ->
+      ssta b e (branch2::pos) tb ->
+      ssta (SBinop (PrimUntyped.UBits2 PrimUntyped.UOr) a b) e pos tb
+  | ssta_binop_or_true_:
+    forall a e pos ta b,
+      ssta a e (branch1::pos) ta ->
+      eval_sact_no_vars r sigma ta = Some (Bits [true]) ->
+      ssta (SBinop (PrimUntyped.UBits2 PrimUntyped.UOr) a b) e pos const_true
+  | ssta_binop_or__false:
+    forall a e pos ta b tb,
+      ssta a e (branch1::pos) ta ->
+      ssta b e (branch2::pos) tb ->
+      eval_sact_no_vars r sigma tb = Some (Bits [false]) ->
+      ssta (SBinop (PrimUntyped.UBits2 PrimUntyped.UOr) a b) e pos ta
+  | ssta_binop_or__true:
+    forall a e pos b tb,
+      ssta b e (branch2::pos) tb ->
+      eval_sact_no_vars r sigma tb = Some (Bits [true]) ->
+      ssta (SBinop (PrimUntyped.UBits2 PrimUntyped.UOr) a b) e pos const_true
+  | ssta_binop_sigma:
+    forall ufn a e pos ta b tb va vb v,
+      ssta a e (branch1::pos) ta ->
+      ssta b e (branch2::pos) tb ->
+      eval_sact_no_vars r sigma ta = Some va ->
+      eval_sact_no_vars r sigma tb = Some vb ->
+      sigma2 ufn va vb = Some v ->
+      ssta (SBinop ufn a b) e pos
+           (SConst v)
+  | ssta_binop_exempted:
+    forall ufn a e pos ta b tb,
+      ssta a e (branch1::pos) ta ->
+      ssta b e (branch2::pos) tb ->
+      ssta (SBinop ufn a b) e pos
+           (SBinop ufn ta tb)
+  | ssta_external_all_exempted:
+    forall ufn a e pos ta,
+      ssta a e (branch1::pos) ta ->
+      ssta (SExternalCall ufn a) e pos
+        (SExternalCall ufn ta)
+  | ssta_id: forall s e pos, ssta s e pos s
+  .
+
+  Lemma ssta_f:
+    forall a e p,
+      ssta a e p (simplify_sact_targeted_aux a e p).
   Proof.
-  Admitted.
+    induction a; simpl; intros; eauto.
+    - constructor.
+    - constructor.
+    - destr.
+      constructor; eauto.
+      destr. 2: constructor; eauto.
+      destr; try now (constructor; eauto).
+      destr; try now (constructor; eauto).
+      repeat destr; try now (constructor; eauto).
+      eapply ssta_if_true; eauto.
+      eapply ssta_if_false; eauto.
+    - destr.
+      eapply ssta_unop_exempted; eauto.
+      repeat destr; try now (constructor; eauto).
+      econstructor; eauto.
+    - destr. econstructor; eauto.
+      destr.
+      repeat destr; try now (constructor; eauto).
+      eapply ssta_binop_sigma; eauto.
+      destr; try now (constructor; eauto).
+      + repeat destr; try now (econstructor; eauto).
+      + repeat destr; try now (econstructor; eauto).
+      + repeat destr; try now (econstructor; eauto).
+      + repeat destr; try now (econstructor; eauto).
+      + repeat destr; try now (econstructor; eauto).
+      + repeat destr; try now (econstructor; eauto).
+      + repeat destr; try now (econstructor; eauto).
+      + repeat destr; try now (econstructor; eauto).
+      + repeat destr; try now (econstructor; eauto).
+      + repeat destr; try now (econstructor; eauto).
+      + repeat destr; try now (econstructor; eauto).
+      + repeat destr; try now (econstructor; eauto).
+      + repeat destr; try now (econstructor; eauto).
+      + repeat destr; try now (econstructor; eauto).
+      + repeat destr; try now (econstructor; eauto).
+      + repeat destr; try now (econstructor; eauto).
+    - econstructor; eauto.
+    - econstructor; eauto.
+  Qed.
+
+  (* Lemma ssta_f: *)
+  (*   forall a e p, *)
+  (*     ssta a e p = simplify_sact_targeted_aux a e p. *)
+  (* Proof. *)
+  (*   induction a; simpl; intros; eauto. *)
+  (*   - destruct (exempted p e) eqn:?. simpl. f_equal; eauto. *)
+  (*     simpl. rewrite IHa1. *)
+  (*     destruct (eval_sact_no_vars); eauto. *)
+  (*     repeat destr; eauto. rewrite IHa2, IHa3; auto. *)
+  (*   - destruct (exempted p e) eqn:?. simpl. f_equal; eauto. *)
+  (*     simpl. rewrite IHa. *)
+  (*     destruct (eval_sact_no_vars); eauto. *)
+  (*   - destruct (exempted p e) eqn:?. simpl. repeat destr; eauto. *)
+  (*     simpl. rewrite IHa1, IHa2. *)
+  (*     destr. unfold opt_bind. symmetry. destr. destr. simpl. *)
+  (*     destruct negate. destruct val_beq_bits eqn:?. apply val_beq_bits_implies_eq in Heqb0. *)
+  (*     destruct (val_beq v v0)eqn:?. auto. apply val_beq_false in Heqb1; congruence. auto. *)
+  (*     destruct val_beq_bits eqn:?. apply val_beq_bits_implies_eq in Heqb0. *)
+  (*     destruct (val_beq v v0)eqn:?. auto. apply val_beq_false in Heqb1; congruence. auto. *)
+  (*     2:{ *)
+  (*       unfold opt_bind. *)
+  (*       destruct (eval_sact_no_vars); eauto. *)
+  (*       destruct (eval_sact_no_vars); eauto. *)
+  (*     } *)
+  (*     2:{ *)
+  (*       unfold opt_bind. *)
+  (*       destruct (eval_sact_no_vars); eauto. *)
+  (*       destruct (eval_sact_no_vars); eauto. *)
+  (*     } *)
+  (*     destr; eauto. *)
+  (*     { *)
+  (*       destruct (eval_sact_no_vars r sigma (simplify_sact_targeted_aux a1 e (branch1::p))) eqn:?; eauto. *)
+  (*       destruct (eval_sact_no_vars r sigma (simplify_sact_targeted_aux a2 e (branch2::p))) eqn:?; eauto. *)
+  (*       repeat destr; eauto. *)
+  (*       repeat destr; eauto. *)
+  (*       repeat destr; eauto. *)
+  (*     } *)
+  (*     { *)
+  (*       destruct (eval_sact_no_vars r sigma (simplify_sact_targeted_aux a1 e (branch1::p))) eqn:?; eauto. *)
+  (*       destruct (eval_sact_no_vars r sigma (simplify_sact_targeted_aux a2 e (branch2::p))) eqn:?; eauto. *)
+  (*       repeat destr; eauto. *)
+  (*       repeat destr; eauto. *)
+  (*       repeat destr; eauto. *)
+  (*     } *)
+  (*     unfold opt_bind. repeat destruct eval_sact_no_vars; eauto. *)
+  (*     unfold opt_bind. repeat destruct eval_sact_no_vars; eauto. *)
+  (*     unfold opt_bind. repeat destruct eval_sact_no_vars; eauto. *)
+  (*     unfold opt_bind. repeat destruct eval_sact_no_vars; eauto. *)
+  (*     unfold opt_bind. repeat destruct eval_sact_no_vars; eauto. *)
+  (*     unfold opt_bind. repeat destruct eval_sact_no_vars; eauto. *)
+  (*     unfold opt_bind. repeat destruct eval_sact_no_vars; eauto. *)
+  (*     unfold opt_bind. repeat destruct eval_sact_no_vars; eauto. *)
+  (*     unfold opt_bind. repeat destruct eval_sact_no_vars; eauto. *)
+  (*     unfold opt_bind. repeat destruct eval_sact_no_vars; eauto. *)
+  (*     unfold opt_bind. repeat destruct eval_sact_no_vars; eauto. *)
+  (*     unfold opt_bind. repeat destruct eval_sact_no_vars; eauto. *)
+  (*   - simpl. rewrite IHa. auto. *)
+  (* Qed. *)
 
   Lemma wt_simplify_sact_targeted:
     forall vss a t,
-    wt_sact R (Sigma:=Sigma) vss a t
-    -> forall e p, wt_sact R (Sigma:=Sigma) vss (simplify_sact_targeted_aux a e p) t.
+      wt_sact R (Sigma:=Sigma) vss a t ->
+      forall ta e p,
+        ssta a e p ta ->
+        wt_sact R (Sigma:=Sigma) vss ta t.
   Proof.
     induction 1; simpl; intros; eauto.
-    - econstructor; eauto.
-    - econstructor; eauto.
-    - destruct (exempted p e).
-      constructor; eauto.
-      destr.
-      exploit (
-        eval_sact_no_vars_wt
-          (reg_t := reg_t) (ext_fn_t := ext_fn_t) (REnv := REnv)
-      ).
-      eauto. eauto. 2: eauto. eauto.
-      intro WT. apply Sact.wt_val_bool in WT. destruct WT; subst.
-      destr; eauto.
-      econstructor; eauto.
-    - assert (
-        wt_sact
-          (Sigma:=Sigma) R vss
-          match
-            eval_sact_no_vars r sigma (simplify_sact_targeted_aux a e p)
-          with
-          | Some x =>
-            match sigma1 ufn x with
-            | Some r => SConst r
-            | None =>
-              SUnop ufn (simplify_sact_targeted_aux a e (p ++ [branch1]))
-            end
-          | None => SUnop ufn (simplify_sact_targeted_aux a e (p ++ [branch1]))
-          end t'
-      ). {
-        destr.
-        exploit (
-          eval_sact_no_vars_wt
-            (reg_t := reg_t) (ext_fn_t := ext_fn_t) (REnv := REnv)
-        ).
-        eauto. eauto. 2: eauto. eauto.
-        intro WT.
-        destr.
-        econstructor; eauto.
-        eapply Wt.wt_unop_sigma1; eauto.
-        econstructor; eauto.
-        econstructor; eauto.
-      }
-      destruct (exempted p e) eqn:eq.
-      + destr_in H1.
-        * destr_in H1; econstructor; eauto; eauto.
-        * econstructor; eauto; eauto.
-      + destr; auto.
-        * repeat destr_in H1.
-          ** exploit IHwt_sact. intro.
-             repeat destr_in H1.
-  Admitted.
+    - inv H0. econstructor; eauto.
+    - inv H0. econstructor; eauto.
+    - inv H2. eauto. eauto. econstructor; eauto. econstructor; eauto.
+    - inv H1.
+      + constructor. eapply Wt.wt_unop_sigma1; eauto.
+        eapply eval_sact_no_vars_wt. 4: eauto. all: eauto.
+      + econstructor; eauto.
+      + econstructor; eauto.
+    - inv H2; try (inv H1; [idtac]); eauto.
+      + eapply eval_sact_no_vars_wt in H10; eauto. inv H10.
+        simpl. repeat constructor.
+      + eapply eval_sact_no_vars_wt in H10; eauto. inv H10.
+        simpl. repeat constructor.
+      + eapply eval_sact_no_vars_wt in H10; eauto. inv H10.
+        simpl. repeat constructor.
+      + eapply eval_sact_no_vars_wt in H10; eauto. inv H10.
+        simpl. repeat constructor.
+      + constructor. eapply Wt.wt_binop_sigma1; eauto.
+        eapply eval_sact_no_vars_wt. 4: eauto. all: eauto.
+        eapply eval_sact_no_vars_wt. 4: eauto. all: eauto.
+      + econstructor; eauto.
+      + econstructor; eauto.
+    - inv H0; econstructor; eauto.
+    - inv H; econstructor; eauto.
+  Qed.
+
+  Require Operations.
+  Lemma simplify_sact_targeted_correct:
+    forall vvs (WTV: wt_vvs R (Sigma:=Sigma) vvs) a e p ta
+           (SSTA: ssta a e p ta)
+           n res t
+           (WTa: wt_sact (Sigma:=Sigma) R vvs a t)
+           (EVAL: eval_sact vvs a n = Some res),
+      eval_sact vvs ta n = Some res.
+  Proof.
+    induction 2; simpl; intros; eauto.
+    - inv WTa.
+      destruct n; simpl in EVAL;
+        unfold opt_bind in EVAL;
+        repeat destr_in EVAL; try congruence.
+      eapply IHSSTA2; eauto.
+      eapply Operations.eval_sact_more_fuel; eauto.
+      eapply eval_sact_eval_sact_no_vars in H; eauto. congruence.
+    - inv WTa.
+      destruct n; simpl in EVAL;
+        unfold opt_bind in EVAL;
+        repeat destr_in EVAL; try congruence.
+      eapply eval_sact_eval_sact_no_vars in H; eauto. congruence.
+      eapply IHSSTA2; eauto.
+      eapply Operations.eval_sact_more_fuel; eauto.
+    - inv WTa.
+      destruct n; simpl in EVAL;
+        unfold opt_bind in EVAL;
+        repeat (destr_in EVAL; try congruence; [idtac]).
+      congruence.
+      simpl.
+      erewrite IHSSTA1; eauto. simpl. destr; eauto.
+    - inv WTa.
+      destruct n; simpl in EVAL;
+        unfold opt_bind in EVAL;
+        repeat (destr_in EVAL; try congruence; [idtac]).
+      congruence.
+      simpl.
+      eapply eval_sact_eval_sact_no_vars in H; eauto. congruence.
+    - inv WTa.
+      destruct n; simpl in EVAL;
+        unfold opt_bind in EVAL;
+        repeat (destr_in EVAL; try congruence; [idtac]).
+      congruence.
+      simpl.
+      erewrite IHSSTA; eauto.
+    - inv WTa.
+      destruct n; simpl in EVAL;
+        unfold opt_bind in EVAL;
+        repeat (destr_in EVAL; try congruence; [idtac]).
+      congruence. inv EVAL.
+      eapply IHSSTA1 in Heqo; eauto.
+      eapply eval_sact_eval_sact_no_vars in Heqo; eauto. inv Heqo.
+      erewrite IHSSTA2; eauto.
+      eapply eval_sact_no_vars_wt in H; eauto. 2: eapply wt_simplify_sact_targeted. 3: eauto.
+      2: eauto. inv H. inv H6.
+      eapply eval_sact_wt in Heqo0 as WTv2; eauto. inv WTv2.
+      destruct v2; simpl in H1; try congruence.
+      destruct v2; simpl in H1; try congruence.
+      simpl bitwise.
+      eapply Operations.eval_sact_more_fuel. eauto. auto.
+    - inv WTa.
+      destruct n; simpl in EVAL;
+        unfold opt_bind in EVAL;
+        repeat (destr_in EVAL; try congruence; [idtac]).
+      congruence. inv EVAL.
+      eapply IHSSTA in Heqo; eauto.
+      eapply eval_sact_eval_sact_no_vars in Heqo; eauto. inv Heqo.
+      eapply eval_sact_no_vars_wt in H; eauto. 2: eapply wt_simplify_sact_targeted. 3: eauto.
+      2: eauto. inv H. inv H6.
+      eapply eval_sact_wt in Heqo0 as WTv2; eauto. inv WTv2.
+      destruct v2; simpl in H1; try congruence.
+      destruct v2; simpl in H1; try congruence.
+      simpl bitwise.
+      reflexivity.
+    - inv WTa.
+      destruct n; simpl in EVAL;
+        unfold opt_bind in EVAL;
+        repeat (destr_in EVAL; try congruence; [idtac]).
+      congruence. inv EVAL.
+      eapply IHSSTA2 in Heqo0; eauto.
+      eapply eval_sact_eval_sact_no_vars in Heqo0; eauto. inv Heqo0.
+      erewrite IHSSTA1; eauto.
+      eapply eval_sact_no_vars_wt in H; eauto. 2: eapply wt_simplify_sact_targeted. 3: eauto.
+      2: eauto. inv H. inv H6.
+      eapply eval_sact_wt in Heqo as WTv1; eauto. inv WTv1.
+      destruct v1; simpl in H1; try congruence.
+      destruct v1; simpl in H1; try congruence.
+      simpl bitwise. rewrite andb_true_r.
+      eapply Operations.eval_sact_more_fuel. eauto. auto.
+    - inv WTa.
+      destruct n; simpl in EVAL;
+        unfold opt_bind in EVAL;
+        repeat (destr_in EVAL; try congruence; [idtac]).
+      congruence. inv EVAL.
+      eapply IHSSTA in Heqo0; eauto.
+      eapply eval_sact_eval_sact_no_vars in Heqo0; eauto. inv Heqo0.
+      eapply eval_sact_no_vars_wt in H; eauto. 2: eapply wt_simplify_sact_targeted. 3: eauto.
+      2: eauto. inv H. inv H6.
+      eapply eval_sact_wt in Heqo as WTv1; eauto. inv WTv1.
+      destruct v1; simpl in H1; try congruence.
+      destruct v1; simpl in H1; try congruence.
+      simpl bitwise. rewrite andb_false_r.
+      reflexivity.
+    - inv WTa.
+      destruct n; simpl in EVAL;
+        unfold opt_bind in EVAL;
+        repeat (destr_in EVAL; try congruence; [idtac]).
+      congruence. inv EVAL.
+      eapply IHSSTA1 in Heqo; eauto.
+      eapply eval_sact_eval_sact_no_vars in Heqo; eauto. inv Heqo.
+      erewrite IHSSTA2; eauto.
+      eapply eval_sact_no_vars_wt in H; eauto. 2: eapply wt_simplify_sact_targeted. 3: eauto.
+      2: eauto. inv H. inv H6.
+      eapply eval_sact_wt in Heqo0 as WTv2; eauto. inv WTv2.
+      destruct v2; simpl in H1; try congruence.
+      destruct v2; simpl in H1; try congruence.
+      simpl bitwise.
+      eapply Operations.eval_sact_more_fuel. eauto. auto.
+    - inv WTa.
+      destruct n; simpl in EVAL;
+        unfold opt_bind in EVAL;
+        repeat (destr_in EVAL; try congruence; [idtac]).
+      congruence. inv EVAL.
+      eapply IHSSTA in Heqo; eauto.
+      eapply eval_sact_eval_sact_no_vars in Heqo; eauto. inv Heqo.
+      eapply eval_sact_no_vars_wt in H; eauto. 2: eapply wt_simplify_sact_targeted. 3: eauto.
+      2: eauto. inv H. inv H6.
+      eapply eval_sact_wt in Heqo0 as WTv2; eauto. inv WTv2.
+      destruct v2; simpl in H1; try congruence.
+      destruct v2; simpl in H1; try congruence.
+      simpl bitwise.
+      reflexivity.
+    - inv WTa.
+      destruct n; simpl in EVAL;
+        unfold opt_bind in EVAL;
+        repeat (destr_in EVAL; try congruence; [idtac]).
+      congruence. inv EVAL.
+      eapply IHSSTA2 in Heqo0; eauto.
+      eapply eval_sact_eval_sact_no_vars in Heqo0; eauto. inv Heqo0.
+      erewrite IHSSTA1; eauto.
+      eapply eval_sact_no_vars_wt in H; eauto. 2: eapply wt_simplify_sact_targeted. 3: eauto.
+      2: eauto. inv H. inv H6.
+      eapply eval_sact_wt in Heqo as WTv1; eauto. inv WTv1.
+      destruct v1; simpl in H1; try congruence.
+      destruct v1; simpl in H1; try congruence.
+      simpl bitwise. rewrite orb_false_r.
+      eapply Operations.eval_sact_more_fuel. eauto. auto.
+    - inv WTa.
+      destruct n; simpl in EVAL;
+        unfold opt_bind in EVAL;
+        repeat (destr_in EVAL; try congruence; [idtac]).
+      congruence. inv EVAL.
+      eapply IHSSTA in Heqo0; eauto.
+      eapply eval_sact_eval_sact_no_vars in Heqo0; eauto. inv Heqo0.
+      eapply eval_sact_no_vars_wt in H; eauto. 2: eapply wt_simplify_sact_targeted. 3: eauto.
+      2: eauto. inv H. inv H6.
+      eapply eval_sact_wt in Heqo as WTv1; eauto. inv WTv1.
+      destruct v1; simpl in H1; try congruence.
+      destruct v1; simpl in H1; try congruence.
+      simpl bitwise. rewrite orb_true_r.
+      reflexivity.
+    - inv WTa.
+      destruct n; simpl in EVAL;
+        unfold opt_bind in EVAL;
+        repeat (destr_in EVAL; try congruence; [idtac]).
+      congruence. inv EVAL.
+      eapply IHSSTA1 in Heqo; eauto.
+      eapply IHSSTA2 in Heqo0; eauto.
+      eapply eval_sact_eval_sact_no_vars in Heqo; eauto.
+      eapply eval_sact_eval_sact_no_vars in Heqo0; eauto. subst. simpl. congruence.
+    - inv WTa.
+      destruct n; simpl in EVAL;
+        unfold opt_bind in EVAL;
+        repeat (destr_in EVAL; try congruence; [idtac]).
+      congruence.
+      eapply IHSSTA1 in Heqo; eauto.
+      eapply IHSSTA2 in Heqo0; eauto.
+      simpl. rewrite Heqo, Heqo0. simpl. auto.
+    - inv WTa.
+      destruct n; simpl in EVAL;
+        unfold opt_bind in EVAL;
+        repeat (destr_in EVAL; try congruence; [idtac]).
+      congruence. inv EVAL.
+      simpl.
+      erewrite IHSSTA; eauto.
+      simpl; auto.
+  Qed.
+
+  (* Lemma simpl_sact_targeted_aux_some_p1_p2: *)
+  (*   forall e a p1 ta1 (SSTA1: ssta a e p1 ta1) *)
+  (*          p2 ta2 (SSTA2: ssta a e p2 ta2) v1 v2, *)
+  (*   eval_sact_no_vars r sigma ta1 = Some v1 *)
+  (*   -> eval_sact_no_vars r sigma ta2 = Some v2 *)
+  (*   -> v1 = v2. *)
+  (* Proof. *)
+  (*   induction 1; simpl; intros; eauto. *)
+  (* Qed. *)
 
   Lemma simplify_sact_wt_sact_targeted_ok':
     forall vvs a t (WTS: wt_sact (Sigma := Sigma) R vvs a t) e,
     wt_sact (Sigma := Sigma) R vvs (simplify_sact_targeted a e) t.
-  Proof. intros. apply wt_simplify_sact_targeted. eauto. Qed.
+  Proof. intros. eapply wt_simplify_sact_targeted. eauto. eapply ssta_f. Qed.
 
   Lemma simplify_sact_targeted_reachable_vars_ok:
-    forall vvs v s e p (RV: reachable_var vvs (simplify_sact_targeted_aux s e p) v),
+    forall vvs v s e p ts (SSTA: ssta s e p ts)
+           (RV: reachable_var vvs ts v),
     reachable_var vvs s v.
   Proof.
-    induction s; intros; simpl in *; eauto.
-    - repeat (destr_in RV); eauto;
-        try (
-          inv RV;
-          try (eapply reachable_var_if_cond; eauto; fail);
-          try (eapply reachable_var_if_true; eauto; fail);
-          try (eapply reachable_var_if_false; eauto; fail);
-          fail); subst.
-      + econstructor.
-        unfold simplify_sact_targeted in *. simpl in *.
-  Admitted.
+    induction 1; intros; simpl in *; eauto.
+    - eapply reachable_var_if_true; eauto.
+    - eapply reachable_var_if_false; eauto.
+    - inv RV.
+      eapply reachable_var_if_cond; eauto.
+      eapply reachable_var_if_true; eauto.
+      eapply reachable_var_if_false; eauto.
+    - inv RV.
+    - inv RV; econstructor; eauto.
+    - eapply reachable_var_binop2; eauto.
+    - inv RV.
+    - eapply reachable_var_binop1; eauto.
+    - inv RV.
+    - eapply reachable_var_binop2; eauto.
+    - inv RV.
+    - eapply reachable_var_binop1; eauto.
+    - inv RV.
+    - inv RV.
+    - inv RV.
+      eapply reachable_var_binop1; eauto.
+      eapply reachable_var_binop2; eauto.
+    - inv RV; econstructor; eauto.
+  Qed.
 
   Lemma simplify_sact_targeted_interp_sact_ok':
     forall a v vvs (WTVVS: wt_vvs (Sigma := Sigma) R vvs) t e
@@ -347,44 +747,190 @@ Section SimplifyTargeted.
     eapply eval_sact_interp_sact.
     unfold simplify_sact_targeted.
     erewrite simplify_sact_targeted_correct; eauto.
+    eapply ssta_f.
   Qed.
-
+  
   Lemma simplify_sact_targeted_var_in_sact_ok':
-    forall s v e (VIS: var_in_sact (simplify_sact_targeted s e) v),
+    forall s e p ts (SSTA: ssta s e p ts) v
+           (VIS: var_in_sact ts v),
     var_in_sact s v.
   Proof.
-    unfold simplify_sact_targeted.
-    intros.
-    induction s; try (eauto; fail).
-    - simpl in VIS. repeat (destr_in VIS); try (
-        inv VIS; try (apply var_in_if_cond; eauto; fail);
-        try (apply var_in_if_true; eauto; fail);
-        try (apply var_in_if_false; eauto; fail);
-        fail).
-  Admitted.
+    induction 1; intros; simpl in *; eauto.
+    - eapply var_in_if_true; eauto.
+    - eapply var_in_if_false; eauto.
+    - inv VIS.
+      eapply var_in_if_cond; eauto.
+      eapply var_in_if_true; eauto.
+      eapply var_in_if_false; eauto.
+    - inv VIS.
+    - inv VIS; econstructor; eauto.
+    - eapply var_in_sact_binop_2; eauto.
+    - inv VIS.
+    - eapply var_in_sact_binop_1; eauto.
+    - inv VIS.
+    - eapply var_in_sact_binop_2; eauto.
+    - inv VIS.
+    - eapply var_in_sact_binop_1; eauto.
+    - inv VIS.
+    - inv VIS.
+    - inv VIS.
+      eapply var_in_sact_binop_1; eauto.
+      eapply var_in_sact_binop_2; eauto.
+    - inv VIS; econstructor; eauto.
+  Qed.
 
   Lemma simplify_sact_targeted_interp_sact_ok:
     forall
       vvs (WTVVS: wt_vvs (Sigma := Sigma) R vvs)
-      (VVSSV: vvs_smaller_variables vvs) a v e
+      (VVSSV: vvs_smaller_variables vvs) a e p ta
+      (SSTA: ssta a e p ta) v
       (EV_INIT:
-        interp_sact (sigma := sigma) REnv r vvs (simplify_sact_targeted a e) v)
+        interp_sact (sigma := sigma) REnv r vvs ta v)
       t (WTS: wt_sact (Sigma := Sigma) R vvs a t),
     interp_sact (sigma := sigma) REnv r vvs a v.
   Proof.
-    unfold simplify_sact_targeted. induction a; simpl; intros; eauto; inv WTS.
-  Admitted.
+    induction 3; simpl; intros; (try (inv WTS; [idtac])); eauto.
+    - econstructor; eauto.
+      eapply eval_sact_no_vars_interp in H; eauto.
+      simpl. eauto.
+    - econstructor; eauto.
+      eapply eval_sact_no_vars_interp in H; eauto.
+      simpl. eauto.
+    - inv EV_INIT. econstructor; eauto.
+      destr; eauto.
+    - inv EV_INIT. econstructor; eauto.
+      eapply eval_sact_no_vars_interp in H; eauto.
+    - inv EV_INIT. econstructor; eauto.
+    - eapply eval_sact_no_vars_interp in H; eauto.
+      econstructor; eauto.
+      eapply interp_sact_wt in H; eauto. 3: eapply wt_simplify_sact_targeted. 4: eauto. 3: eauto.
+      inv H. inv H6.
+      eapply interp_sact_wt in EV_INIT; eauto. 3: eapply wt_simplify_sact_targeted. 4: eauto. 3: eauto.
+      destruct (Sact.wt_val_bool _ EV_INIT). subst. simpl. reflexivity.
+      apply vvs_range_max_var.
+      apply vvs_range_max_var.
+    - inv EV_INIT.
+      exploit @eval_sact_no_vars_wt. 4: apply H. 1-2: eauto. eapply wt_simplify_sact_targeted. 2: eauto. eauto.
+      intro A; inv A. inv H6. simpl in *.
+      edestruct (@wt_sact_interp) as (? & IS & WTv). 6: apply H5. all: eauto. apply vvs_range_max_var.
+      econstructor; eauto.
+      eapply IHSSTA.
+      eapply eval_sact_no_vars_interp; eauto. eauto.
+      destruct (Sact.wt_val_bool _ WTv). subst. simpl. reflexivity.
+    - eapply eval_sact_no_vars_interp in H; eauto.
+      econstructor; eauto.
+      eapply interp_sact_wt in H; eauto. 3: eapply wt_simplify_sact_targeted. 4: eauto. 3: eauto.
+      inv H. inv H6.
+      eapply interp_sact_wt in EV_INIT; eauto. 3: eapply wt_simplify_sact_targeted. 4: eauto. 3: eauto.
+      destruct (Sact.wt_val_bool _ EV_INIT). subst. simpl. rewrite andb_true_r; reflexivity.
+      apply vvs_range_max_var.
+      apply vvs_range_max_var.
+    - inv EV_INIT.
+      exploit @eval_sact_no_vars_wt. 4: apply H. 1-2: eauto. eapply wt_simplify_sact_targeted. 2: eauto. eauto.
+      intro A; inv A. inv H6. simpl in *.
+      edestruct (@wt_sact_interp) as (? & IS & WTv). 6: apply H3. all: eauto. apply vvs_range_max_var.
+      econstructor; eauto.
+      eapply IHSSTA.
+      eapply eval_sact_no_vars_interp; eauto. eauto.
+      destruct (Sact.wt_val_bool _ WTv). subst. simpl. rewrite andb_false_r. reflexivity.
+    - eapply eval_sact_no_vars_interp in H; eauto.
+      econstructor; eauto.
+      eapply interp_sact_wt in H; eauto. 3: eapply wt_simplify_sact_targeted. 4: eauto. 3: eauto.
+      inv H. inv H6.
+      eapply interp_sact_wt in EV_INIT; eauto. 3: eapply wt_simplify_sact_targeted. 4: eauto. 3: eauto.
+      destruct (Sact.wt_val_bool _ EV_INIT). subst. simpl. reflexivity.
+      apply vvs_range_max_var.
+      apply vvs_range_max_var.
+    - inv EV_INIT.
+      exploit @eval_sact_no_vars_wt. 4: apply H. 1-2: eauto. eapply wt_simplify_sact_targeted. 2: eauto. eauto.
+      intro A; inv A. inv H6. simpl in *.
+      edestruct (@wt_sact_interp) as (? & IS & WTv). 6: apply H5. all: eauto. apply vvs_range_max_var.
+      econstructor; eauto.
+      eapply IHSSTA.
+      eapply eval_sact_no_vars_interp; eauto. eauto.
+      destruct (Sact.wt_val_bool _ WTv). subst. simpl. reflexivity.
+    - eapply eval_sact_no_vars_interp in H; eauto.
+      econstructor; eauto.
+      eapply interp_sact_wt in H; eauto. 3: eapply wt_simplify_sact_targeted. 4: eauto. 3: eauto.
+      inv H. inv H6.
+      eapply interp_sact_wt in EV_INIT; eauto. 3: eapply wt_simplify_sact_targeted. 4: eauto. 3: eauto.
+      destruct (Sact.wt_val_bool _ EV_INIT). subst. simpl. rewrite orb_false_r; reflexivity.
+      apply vvs_range_max_var.
+      apply vvs_range_max_var.
+    - inv EV_INIT.
+      exploit @eval_sact_no_vars_wt. 4: apply H. 1-2: eauto. eapply wt_simplify_sact_targeted. 2: eauto. eauto.
+      intro A; inv A. inv H6. simpl in *.
+      edestruct (@wt_sact_interp) as (? & IS & WTv). 6: apply H3. all: eauto. apply vvs_range_max_var.
+      econstructor; eauto.
+      eapply IHSSTA.
+      eapply eval_sact_no_vars_interp; eauto. eauto.
+      destruct (Sact.wt_val_bool _ WTv). subst. simpl. rewrite orb_true_r. reflexivity.
+    - eapply eval_sact_no_vars_interp in H; eauto.
+      eapply eval_sact_no_vars_interp in H0; eauto.
+      eapply IHSSTA1 in H; eauto.
+      eapply IHSSTA2 in H0; eauto.
+      inv EV_INIT. econstructor; eauto. 
+    - inv EV_INIT. econstructor; eauto.
+    - inv EV_INIT. econstructor; eauto.
+  Qed.
+
+  (* Definition simplify_sf_targeted *)
+  (*   (sf: simple_form) (exemptions: list (list position)) *)
+  (* := {| *)
+  (*   final_values := final_values sf; *)
+  (*   vars := *)
+  (*     fst ( *)
+  (*       PTree.fold *)
+  (*       (fun *)
+  (*         (acc: ((PTree.tree (type * SimpleForm.sact)) * list (list position))) *)
+  (*         elt (val: (type * SimpleForm.sact)) *)
+  (*       => *)
+  (*         let '(tree, acc_exs) := acc in *)
+  (*         let exs: list position := List.hd [] acc_exs in *)
+  (*         let res := simplify_sact_targeted (snd val) exs in *)
+  (*         (PTree.set elt (fst val, res) tree, tl acc_exs)) *)
+  (*       (vars sf) *)
+  (*       (PTree.empty (type * SimpleForm.sact), exemptions)) *)
+  (*   |}. *)
+
+
+  Definition simplify_sf_targeted
+    (sf: simple_form) (exemptions: PTree.t (list position))
+  := {|
+    final_values := final_values sf;
+    vars :=
+      PTree.map (fun k '(t, s) =>
+                   let exs :=
+                     match PTree.get k exemptions with
+                       Some l => l
+                     | _ => []
+                     end in
+                   (t, simplify_sact_targeted s exs)
+        )
+        (vars sf)
+    |}.
 
   Lemma sf_eq_simplify_sf_targeted sf:
     forall e,
     wf_sf sf -> sf_eq R Sigma r sigma sf (simplify_sf_targeted sf e).
   Proof.
-  Admitted.
+    intros.
+    eapply sf_eq_mapi.
+    - intros. eapply simplify_sact_targeted_interp_sact_ok; eauto. eapply ssta_f.
+    - intros; eapply simplify_sact_targeted_interp_sact_ok'; eauto.
+    - intros; eapply simplify_sact_wt_sact_targeted_ok'; eauto.
+    - intros; eapply simplify_sact_targeted_var_in_sact_ok'; eauto. eapply ssta_f.
+    - eauto.
+  Qed.
 
   Lemma wf_sf_simplify_sf_targeted:
     forall sf, wf_sf sf -> forall e, wf_sf (simplify_sf_targeted sf e).
   Proof.
-  Admitted.
+    intros.
+    eapply wf_fi; eauto.
+    - intros; eapply simplify_sact_wt_sact_targeted_ok'; eauto.
+    - intros; eapply simplify_sact_targeted_var_in_sact_ok'; eauto. eapply ssta_f.
+  Qed.
 
   Lemma simplify_sf_targeted_interp_cycle_ok:
     forall reg sf e,
